src/LLBC_plus.v
@@ -1,7 +1,7 @@
 (** * Mechanized_LLBC.LLBC_plus : Semantics of LLBC+. *)
 (** All of the judgement are identical to LLBC##, except the evaluation of statements. *)
 From stdpp Require Import fin_maps.
-Require Import lang SimulationUtils Symbolic_states Symbolic_relations.
+Require Import base lang Symbolic_states.
 Require Import LLBC_sharp.
 
 Declare Scope llbc_plus_scope.
